Launchbury/CoCallCardinality.thy
@@ -1,0 +1,56 @@
+theory CoCallCardinality
+imports FTreeCardinality CoCallAnalysis
+begin
+
+definition aeFtree :: "AEnv \<Rightarrow> var ftree"
+  where "aeFtree ae = many_among (edom ae)"
+
+lemma cont_aeFtree[THEN cont_compose, cont2cont, simp]:
+  "cont aeFtree"
+  sorry
+
+
+lemma  valid_lists_downset_aux:
+  "xs \<in> valid_lists CoCalls \<Longrightarrow> butlast xs \<in> valid_lists CoCalls"
+  by (induction xs) (auto dest: in_set_butlastD)
+
+
+lift_definition ccFTree :: "CoCalls \<Rightarrow> var ftree" is "\<lambda> G. valid_lists G" 
+  by (auto intro: valid_lists_downset_aux)
+
+lemma cont_ccFTree[THEN cont_compose, cont2cont, simp]:
+  "cont ccFTree"
+  sorry
+
+locale CoCallCardinality = CoCallAnalysis + CoCallAnalyisHeap + CorrectArityAnalysisLet'
+begin
+
+definition Fexp :: "exp \<Rightarrow> Arity \<rightarrow> var ftree"
+  where "Fexp e = (\<Lambda> a. ccFTree (ccExp e\<cdot>a) \<inter>\<inter> aeFtree (Aexp e\<cdot>a))"
+
+lemma Fexp_simp: "Fexp e\<cdot>a = ccFTree (ccExp e\<cdot>a) \<inter>\<inter> aeFtree (Aexp e\<cdot>a)"
+  unfolding Fexp_def by (rule beta_cfun) (intro cont2cont)
+
+definition Fheap :: "heap \<Rightarrow> exp \<Rightarrow> Arity \<rightarrow> var ftree"
+  where "Fheap \<Gamma> e = (\<Lambda> a. ccFTree (ccHeap \<Gamma> e\<cdot>a) \<inter>\<inter> aeFtree (Aheap \<Gamma> e\<cdot>a))"
+
+lemma Fheap_simp: "Fheap \<Gamma> e\<cdot>a = ccFTree (ccHeap \<Gamma> e\<cdot>a) \<inter>\<inter> aeFtree (Aheap \<Gamma> e\<cdot>a)"
+  unfolding Fheap_def by (rule beta_cfun) (intro cont2cont)
+
+sublocale FutureAnalysis Fexp.
+
+sublocale FutureAnalysisCarrier Fexp
+  apply default
+  sorry
+
+sublocale FutureAnalysisCorrect Fexp
+  apply default
+  sorry
+
+
+sublocale FutureAnalysisCardinalityHeap Fexp Aexp Aheap Fheap
+  apply default
+  sorry
+
+end
+
