ROOT
@@ -36,13 +36,14 @@ session Arity (AFP) in "Launchbury" = "HOLCF-Nominal2" +
     "ArityAnalysisImpl"
     "TrivialArityAnal"
     "ArityEtaExpand"
-    "FutureEtaExpand"
+    "CardinalityEtaExpand"
     "EtaExpansionSestoft"
     "DeadCodeRemovalCorrect"
     "DeadCodeRemoval2Correct"
     "DeadCodeRemoval2CorrectSestoft"
     "RedsImprovesArityAnalysis"
     "NoCardinalityAnalysis"
+    "FTreeCardinality"
 
 session Nominal2013_1 in "Nominal2-Isabelle2013-1/Nominal" = HOL +
   theories
